feat(chap12): add wp and its lemmas

ConcreteSemanticsChapter12/ConcreteSemantics12_Hoare_Sound_Complete.thy
@@ -2,4 +2,89 @@ theory ConcreteSemantics12_Hoare_Sound_Complete
   imports "~~/src/HOL/IMP/Hoare"
 begin
 
+subsection \<open>Soundness and Completeness\<close>
+
+subsubsection "Soundness"
+
+lemma hoare_sound: "\<turnstile> {P}c{Q}  \<Longrightarrow>  \<Turnstile> {P}c{Q}"
+proof(induction rule: hoare.induct)
+case (Skip P)
+  then show ?case 
+    using hoare_valid_def by auto
+next
+  case (Assign P a x)
+  then show ?case 
+    using hoare_valid_def by auto
+next
+  case (Seq P c\<^sub>1 Q c\<^sub>2 R)
+  then show ?case 
+    using hoare_valid_def by auto
+next
+  case (If P b c\<^sub>1 Q c\<^sub>2)
+  then show ?case 
+    using hoare_valid_def by auto
+next
+  case (While P b c)
+  have "(WHILE b DO c, s) \<Rightarrow> t \<Longrightarrow> P s \<Longrightarrow> P t \<and> \<not> bval b t" for s t 
+  proof(induction "WHILE b DO c" s t rule: big_step_induct)
+    case (WhileFalse s)
+    then show ?case 
+      by simp
+  next
+    case (WhileTrue s\<^sub>1 s\<^sub>2 s\<^sub>3)
+    then show ?case 
+      using While.IH hoare_valid_def by auto
+  qed
+  then show ?case 
+    using hoare_valid_def by auto
+next
+  case (conseq P' P c Q Q')
+  then show ?case 
+    using hoare_valid_def by auto
+qed 
+
+subsubsection "Weakest Precondition"
+
+definition wp :: "com \<Rightarrow> assn \<Rightarrow> assn" where
+"wp c Q = (\<lambda>s. \<forall>t. (c,s) \<Rightarrow> t  \<longrightarrow>  Q t)"
+
+lemma wp_SKIP[simp]: "wp SKIP Q = Q"
+  apply(auto simp: wp_def)
+  done
+
+lemma wp_Ass[simp]: "wp (x::=a) Q = (\<lambda>s. Q(s[a/x]))"
+(*  apply(auto simp: wp_def)
+  done*)
+  by (rule ext) (auto simp: wp_def)
+
+lemma wp_Seq[simp]: "wp (c\<^sub>1;;c\<^sub>2) Q = wp c\<^sub>1 (wp c\<^sub>2 Q)"
+(*  apply(auto simp: wp_def)
+  done*)
+  by (rule ext) (auto simp: wp_def)
+
+lemma wp_If[simp]:
+ "wp (IF b THEN c\<^sub>1 ELSE c\<^sub>2) Q =
+ (\<lambda>s. if bval b s then wp c\<^sub>1 Q s else wp c\<^sub>2 Q s)"
+(*  apply(auto simp: wp_def)
+  done*)
+  by (rule ext) (auto simp: wp_def)
+
+lemma wp_While_If:
+ "wp (WHILE b DO c) Q s =
+  wp (IF b THEN c;;WHILE b DO c ELSE SKIP) Q s"
+(*  apply(auto simp: wp_def)
+  by (simp add: while_unfold)*)
+  unfolding wp_def by (metis unfold_while)
+
+lemma wp_While_True[simp]: "bval b s \<Longrightarrow>
+  wp (WHILE b DO c) Q s = wp (c;; WHILE b DO c) Q s"
+(*    apply(auto simp: wp_def)
+  done*)
+  by (auto simp: wp_While_If)
+
+lemma wp_While_False[simp]: "\<not> bval b s \<Longrightarrow> wp (WHILE b DO c) Q s = Q s"
+(*    apply(auto simp: wp_def)
+  done*)
+  by (auto simp: wp_While_If)
+
 end
